security-monitor/src/core/memory_layout/non_confidential_memory_address.rs
@@ -16,20 +16,19 @@ use pointers_utility::ptr_byte_add_mut;
 #[rr::exists("MEMORY_CONFIG")]
 #[rr::invariant(#iris "once_status \"MEMORY_LAYOUT\" (Some MEMORY_CONFIG)")]
 /// Invariant: The address is in non-confidential memory.
-#[rr::invariant("(MEMORY_CONFIG.(non_conf_start).2 ≤ l.2 < MEMORY_CONFIG.(non_conf_end).2)%Z")]
+#[rr::invariant("(MEMORY_CONFIG.(non_conf_start).(loc_a) ≤ l.(loc_a) < MEMORY_CONFIG.(non_conf_end).(loc_a))%Z")]
 pub struct NonConfidentialMemoryAddress(#[rr::field("l")] *mut usize);
 
 #[rr::context("onceG Σ memory_layout")]
 impl NonConfidentialMemoryAddress {
     /// Constructs an address in a non-confidential memory. Returns error if the address is outside non-confidential
     /// memory.
-    #[rr::trust_me]
     #[rr::params("bounds")]
     /// Precondition: The global memory layout has been initialized.
-    #[rr::requires(#iris "once_status \"MEMORY_LAYOUT\" (Some bounds)")]
+    #[rr::requires(#iris "once_initialized π \"MEMORY_LAYOUT\" (Some bounds)")]
     #[rr::ok]
     /// Precondition: The location is in non-confidential memory.
-    #[rr::requires("bounds.(non_conf_start).2 ≤ address.2 < bounds.(non_conf_end).2")]
+    #[rr::requires("bounds.(non_conf_start).(loc_a) ≤ address.(loc_a) < bounds.(non_conf_end).(loc_a)")]
     /// Postcondition: The non-confidential memory address is correctly initialized.
     #[rr::ensures("ret = address")]
     pub fn new(address: *mut usize) -> Result<Self, Error> {
@@ -46,19 +45,20 @@ impl NonConfidentialMemoryAddress {
     ///
     /// The caller must ensure that the address advanced by the offset is still within the non-confidential memory
     /// region.
-    // TODO: can we require the offset to be a multiple of usize?
-    #[rr::only_spec]
-    #[rr::params("MEMORY_CONFIG")]
-    /// Precondition: The offset address is in the given range.
-    #[rr::requires("self.2 + offset_in_bytes < upper_bound.2")]
+    #[rr::params("MEMORY_CONFIG" : "memory_layout")]
     /// Precondition: The global memory layout is initialized.
-    #[rr::requires(#iris "once_status \"MEMORY_LAYOUT\" (Some MEMORY_CONFIG)")]
+    #[rr::requires(#iris "once_initialized π \"MEMORY_LAYOUT\" (Some MEMORY_CONFIG)")]
+    #[rr::ok]
+    /// Precondition: The offset address is in the given range.
+    #[rr::requires("self.(loc_a) + offset_in_bytes < upper_bound.(loc_a)")]
     /// Precondition: The maximum (and thus the offset address) is in the non-confidential memory range.
-    #[rr::requires("upper_bound.2 < MEMORY_CONFIG.(non_conf_end).2")]
+    #[rr::requires("upper_bound.(loc_a) ≤ MEMORY_CONFIG.(non_conf_end).(loc_a)")]
     /// Postcondition: The offset pointer is in the non-confidential memory range.
-    #[rr::returns("Ok(self +ₗ offset_in_bytes)")]
+    #[rr::ensures("ret = self +ₗ offset_in_bytes")]
     pub unsafe fn add(&self, offset_in_bytes: usize, upper_bound: *const usize) -> Result<NonConfidentialMemoryAddress, Error> {
-        let pointer = ptr_byte_add_mut(self.0, offset_in_bytes, upper_bound).map_err(|_| Error::AddressNotInNonConfidentialMemory())?;
+        let memory_layout = MemoryLayout::read();
+        ensure!(upper_bound <= memory_layout.non_confidential_memory_end, Error::AddressNotInNonConfidentialMemory())?;
+        let pointer = ptr_byte_add_mut(self.0, offset_in_bytes, upper_bound).map_err(#[rr::verify] |_| Error::AddressNotInNonConfidentialMemory())?;
         Ok(NonConfidentialMemoryAddress(pointer))
     }
 
@@ -68,6 +68,10 @@ impl NonConfidentialMemoryAddress {
     ///
     /// We need to ensure the pointer is not used by two threads simultaneously. See `ptr::read_volatile` for safety
     /// concerns.
+    #[rr::params("z", "lft_el")]
+    #[rr::unsafe_elctx("[ϝ ⊑ₑ lft_el]")]
+    #[rr::requires(#iris "self ◁ₗ[π, Shared lft_el] #z @ ◁ int usize")]
+    #[rr::returns("z")]
     pub unsafe fn read(&self) -> usize {
         unsafe { self.0.read_volatile() }
     }
@@ -78,6 +82,9 @@ impl NonConfidentialMemoryAddress {
     ///
     /// We need to ensure the pointer is not used by two threads simultaneously. See `ptr::write_volatile` for safety
     /// concerns.
+    #[rr::params("z")]
+    #[rr::requires(#type "self" : "z" @ "int usize")]
+    #[rr::ensures(#type "self" : "value" @ "int usize")]
     pub unsafe fn write(&self, value: usize) {
         unsafe { self.0.write_volatile(value) };
     }
@@ -87,12 +94,9 @@ impl NonConfidentialMemoryAddress {
         self.0
     }
 
-    #[rr::only_spec]
-    #[rr::returns("self.2")]
+    #[rr::returns("self.(loc_a)")]
     pub fn usize(&self) -> usize {
         // TODO: check if we need to expose the pointer.
-        // If not, use addr() instead.
-        // self.0.addr()
-        self.0 as usize
+        self.0.addr()
     }
 }
