security-monitor/src/lib.rs
@@ -24,3 +24,44 @@ mod confidential_flow;
 mod core;
 mod error;
 mod non_confidential_flow;
+
+/// These wrappers serve as a temporary workaround until RefinedRust supports unsized types and in
+/// particular slices: the indexing and iteration methods on `Vec` work by dereferencing to slices,
+/// which currently are not supported by RefinedRust.
+/// For now, we thus create wrappers for these methods to which we can attach RefinedRust
+/// specifications.
+mod rr_wrappers {
+    use alloc::vec::Vec;
+
+    #[rr::only_spec]
+    #[rr::requires("index < length x.cur")]
+    #[rr::exists("γi")]
+    #[rr::returns("(x.cur !!! Z.to_nat index, γi)")]
+    #[rr::observe("x.ghost": "<[Z.to_nat index := PlaceGhost γi]> (<$#> x.cur)")]
+    pub fn vec_index_mut<T>(x: &mut Vec<T>, index: usize) -> &mut T {
+        &mut x[index]
+    }
+
+    #[rr::only_spec]
+    #[rr::requires("index < length x")]
+    #[rr::returns("x !!! Z.to_nat index")]
+    pub fn vec_index<T>(x: &Vec<T>, index: usize) -> &T {
+        &x[index]
+    }
+
+    #[rr::only_spec]
+    #[rr::returns("x")]
+    pub fn vec_iter<T>(x: &Vec<T>) -> core::slice::Iter<'_, T> {
+        x.iter()
+    }
+
+    #[rr::only_spec]
+    #[rr::exists("γs")]
+    #[rr::ensures("length γs = length x.cur")]
+    #[rr::observe("x.ghost": "(PlaceGhost <$> γs) : list (place_rfn {rt_of T})")]
+    #[rr::returns("zip x.cur γs")]
+    pub fn vec_iter_mut<T>(x: &mut Vec<T>) -> core::slice::IterMut<'_, T> {
+        x.iter_mut()
+    }
+
+}
