verification/rust_proofs/ace/proofs/proof_core_page_allocator_allocator_PageAllocator_acquire_page_closure0.v
@@ -1,0 +1,32 @@
+From caesium Require Import lang notation.
+From refinedrust Require Import typing shims.
+From sm.ace.generated Require Import generated_code_ace generated_specs_ace generated_template_core_page_allocator_allocator_PageAllocator_acquire_page_closure0.
+
+Set Default Proof Using "Type".
+
+Section proof.
+Context `{RRGS : !refinedrustGS Σ}.
+
+Lemma core_page_allocator_allocator_PageAllocator_acquire_page_closure0_proof (π : thread_id) :
+  core_page_allocator_allocator_PageAllocator_acquire_page_closure0_lemma π.
+Proof.
+  core_page_allocator_allocator_PageAllocator_acquire_page_closure0_prelude.
+
+  rep <-! liRStep; liShow.
+  (* !start proof(page_allocator.acquire_page) *)
+  apply_update (updateable_copy_lft "ulft3" "ulft_4").
+  rep <-! liRStep; liShow.
+  (* !end proof *)
+
+  all: print_remaining_goal.
+  Unshelve. all: sidecond_solver.
+  Unshelve. all: sidecond_hammer.
+  (* !start proof(page_allocator.acquire_page) *)
+  1-2: congruence.
+  { rename select (if_Ok _ _) into Hok.
+    match type of Hok with if_Ok ?x _ => rename x into maybe_tok end.
+    destruct maybe_tok; simpl in *; solve_goal. }
+  (* !end proof *)
+  Unshelve. all: print_remaining_sidecond.
+Qed.
+End proof.
