verification/rust_proofs/ace/proofs/proof_core_page_allocator_allocator_PageAllocator_add_memory_region.v
@@ -13,30 +13,30 @@ Proof.
   core_page_allocator_allocator_PageAllocator_add_memory_region_prelude.
 
   rep <-! liRStep; liShow.
+  (* !start proof(page_allocator.add_memory_region) *)
   all: match goal with
   | H : ?x `aligned_to` page_size_in_bytes_nat _ |- _ => rename x into larr
   end.
   all: try match goal with
-  | H : ?x = Size4KiB ∨ _.2 + _ ≤ _ |- _ =>
+  | H : ?x = Size4KiB ∨ _.(loc_a) + _ ≤ _ |- _ =>
       rename x into sz_to_allocate;
       rename H into Hsz_bounds
   end.
-
   { (* calling Page::init *)
     apply_update (updateable_split_array larr (page_size_in_bytes_nat sz_to_allocate)).
-    liRStepUntil typed_val_expr.
+    liRStepUntil typed_call.
     apply_update (updateable_reshape_array larr (page_size_in_words_nat sz_to_allocate) bytes_per_addr).
-    liRStepUntil typed_val_expr.
+    liRStepUntil typed_call.
     iRename select (larr ◁ₗ[_, _] _ @ (◁ _))%I into "Harr".
-    iApply fupd_typed_val_expr.
-    iMod (ltype_own_array_subtype_strong _ _ _ _ (int usize) with "[] Harr") as "(% & Harr)"; [done | | | | | ].
+    iApply fupd_typed_call.
+    iMod (ltype_own_array_subtype_strong _ _ _ _ (int usize) _ _ _ (λ _ _, True%I) with "[] Harr") as "(% & _ & Harr)"; [done | | | | | ].
     { shelve_sidecond. }
     { solve_layout_alg. }
     { shelve_sidecond. }
-    { iModIntro. iIntros (??) "Harr". iPoseProof (ty_own_val_array_int_to_int with "Harr") as "$"; last done.
+    { iModIntro. iIntros (??? _) "Harr". 
+      iPoseProof (ty_own_val_array_int_to_int with "Harr") as "(% & $)"; last done.
       shelve_sidecond. }
     iModIntro.
-
     repeat liRStep. }
   repeat liRStep.
 
@@ -44,17 +44,12 @@ Proof.
   Unshelve. all: sidecond_solver.
   Unshelve. all: try lia.
   all: try congruence.
-  - rewrite -page_size_align_is_size /page_size_align.
-    exists (page_size_align_log Size4KiB). lia.
-  - sidecond_hammer.
+  - apply page_size_in_bytes_is_power_of_two.
+  - solve_goal.
   - specialize (page_size_in_bytes_nat_ge x').
     specialize (page_size_in_bytes_nat_in_usize x') as [].
     split; lia.
-  - specialize (page_size_in_bytes_nat_ge x').
-    specialize (page_size_in_bytes_nat_in_usize x') as [].
-    sidecond_hammer.
   - unfold page_size_in_bytes_nat. lia.
-  - specialize (page_size_in_words_nat_ge sz_to_allocate). lia.
   - intros ? Hly1. apply syn_type_has_layout_array_inv in Hly1 as (? & Hly1 & -> & ?).
     apply syn_type_has_layout_int_inv in Hly1 as ->.
     eexists. split; first by apply syn_type_has_layout_int.
@@ -66,7 +61,7 @@ Proof.
   - sidecond_hammer.
   - rewrite page_size_align_is_size. done.
   - rewrite MAX_PAGE_ADDR_unfold /MAX_PAGE_ADDR_def.
-    revert select (¬ memory_region_end.2 > _).
+    revert select (¬ memory_region_end.(loc_a) > _).
     rewrite Hroot_sz. lia.
   - rename select (max_node_size _ = Size128TiB) into Hroot_sz'.
     rewrite Hroot_sz'.
@@ -74,9 +69,10 @@ Proof.
   - rewrite Hroot_sz Hroot_base.
     split; simpl.
     + lia.
-    + revert select (larr.2 + _ ≤ MAX_PAGE_ADDR). rewrite MAX_PAGE_ADDR_unfold /MAX_PAGE_ADDR_def. lia.
+    + revert select (larr.(loc_a) + _ ≤ MAX_PAGE_ADDR). rewrite MAX_PAGE_ADDR_unfold /MAX_PAGE_ADDR_def. lia.
   - apply aligned_to_offset; first done.
     solve_goal.
+  (* !end proof *)
 
   all: sidecond_hammer.
   Unshelve. all: print_remaining_sidecond.
