verification/rust_proofs/ace/proofs/proof_core_page_allocator_allocator_PageAllocator_find_largest_page_size.v
@@ -12,19 +12,20 @@ Lemma core_page_allocator_allocator_PageAllocator_find_largest_page_size_proof (
 Proof.
   core_page_allocator_allocator_PageAllocator_find_largest_page_size_prelude.
 
-  rep liRStep; liShow. 
-  1: match goal with 
-  | H : capture_address_ `aligned_to` page_size_in_bytes_nat ?x, 
-    H' : page_size_smaller ?x = Some ?x' |- _ => 
+  (* !start proof(page_allocator.find_largest_page_size) *)
+  rep liRStep; liShow.
+  1: match goal with
+  | H : capture_address_ `aligned_to` page_size_in_bytes_nat ?x,
+    H' : page_size_smaller ?x = Some ?x' |- _ =>
       rename x into sz_aligned;
       rename x' into sz_aligned_smaller;
       rename H' into Hsmaller
   end.
   1: rewrite Hsmaller.
   all: rep liRStep; liShow.
-  1: match goal with 
-  | H : address `aligned_to` page_size_in_bytes_nat ?x, 
-    H' : page_size_smaller ?x = Some ?x' |- _ => 
+  1: match goal with
+  | H : address `aligned_to` page_size_in_bytes_nat ?x,
+    H' : page_size_smaller ?x = Some ?x' |- _ =>
       rename x into sz_aligned;
       rename x' into sz_aligned_smaller;
       rename H' into Hsmaller
@@ -36,13 +37,14 @@ Proof.
   Unshelve. all: sidecond_solver.
   Unshelve. all: sidecond_hammer.
 
-  all: try match goal with 
+  all: try match goal with
     | H : _ `aligned_to` page_size_in_bytes_nat ?x |- _ =>
         rename x into sz';
         specialize (page_size_in_bytes_nat_ge sz') as ?
     end.
   all: try lia.
   all: by eapply address_aligned_to_page_size_smaller.
+  (* !end proof *)
 
   Unshelve. all: print_remaining_sidecond.
 (*Qed.*)
