verification/rust_proofs/ace/proofs/proof_core_page_allocator_allocator_PageAllocator_release_pages.v
@@ -1,0 +1,40 @@
+From caesium Require Import lang notation.
+From refinedrust Require Import typing shims.
+From sm.ace.generated Require Import generated_code_ace generated_specs_ace generated_template_core_page_allocator_allocator_PageAllocator_release_pages.
+
+Set Default Proof Using "Type".
+
+Section proof.
+Context `{RRGS : !refinedrustGS Σ}.
+
+Lemma core_page_allocator_allocator_PageAllocator_release_pages_proof (π : thread_id) :
+  core_page_allocator_allocator_PageAllocator_release_pages_lemma π.
+Proof.
+  core_page_allocator_allocator_PageAllocator_release_pages_prelude.
+
+  (* !start proof(page_allocator.release_pages) *)
+  rep <-! liRStep; liShow.
+  (* TODO: lots of spurious lifetimes, due to latebound instantiation (see #27) *)
+  apply_update (updateable_copy_lft "vlft3" "static").
+  rep <-! liRStep; liShow.
+  apply_update (updateable_copy_lft "vlft10" "vlft5").
+  rep <-! liRStep; liShow.
+  apply_update (updateable_copy_lft "vlft12" "vlft5").
+  rep <-! liRStep; liShow.
+  apply_update (updateable_copy_lft "vlft14" "vlft5").
+  rep <-! liRStep; liShow.
+  apply_update (updateable_copy_lft "vlft16" "vlft5").
+  rep <-! liRStep; liShow.
+  rep <- 2 liRStep; liShow.
+  { rep liRStep.
+    unfold once_initialized. rep liRStep. }
+  rep liRStep.
+  (* !end proof *)
+
+
+  all: print_remaining_goal.
+  Unshelve. all: sidecond_solver.
+  Unshelve. all: sidecond_hammer.
+  Unshelve. all: print_remaining_sidecond.
+Qed.
+End proof.
