verification/rust_proofs/ace/proofs/proof_core_page_allocator_allocator_PageAllocator_release_pages_closure0.v
@@ -1,0 +1,43 @@
+From caesium Require Import lang notation.
+From refinedrust Require Import typing shims.
+From sm.ace.generated Require Import generated_code_ace generated_specs_ace generated_template_core_page_allocator_allocator_PageAllocator_release_pages_closure0.
+
+Set Default Proof Using "Type".
+
+Section proof.
+Context `{RRGS : !refinedrustGS Σ}.
+
+Lemma core_page_allocator_allocator_PageAllocator_release_pages_closure0_proof (π : thread_id) :
+  core_page_allocator_allocator_PageAllocator_release_pages_closure0_lemma π.
+Proof.
+  core_page_allocator_allocator_PageAllocator_release_pages_closure0_prelude.
+
+  rep <-! liRStep; liShow.
+  (* !start proof(page_allocator.release_pages) *)
+  apply_update (updateable_copy_lft "ulft2" "ulft_3").
+  rep liRStep; liShow.
+  (* !end proof *)
+
+  all: print_remaining_goal.
+  Unshelve. all: sidecond_solver.
+  Unshelve. all: sidecond_hammer.
+  (* !start proof(page_allocator.release_pages) *)
+  all: try congruence.
+  all: clear_layout.
+  - rename select (max_node_size root_node = Size128TiB) into Hsz_root.
+    rewrite Hsz_root. solve_goal.
+  - rewrite /page_within_range.
+    rewrite Hroot_base.
+    simpl.
+    split. { lia. }
+    rename select (_ ≤ MAX_PAGE_ADDR) into Hbounds.
+    etrans; first apply Hbounds.
+    rewrite MAX_PAGE_ADDR_unfold /MAX_PAGE_ADDR_def.
+    rename select (max_node_size _ = max_node_size root_node) into Hsz.
+    rename select (max_node_size root_node = Size128TiB) into Hsz'.
+    rewrite Hsz Hsz'. lia.
+  (* !end proof *)
+
+  Unshelve. all: print_remaining_sidecond.
+Qed.
+End proof.
