verification/rust_proofs/ace/proofs/proof_core_page_allocator_allocator_PageStorageTreeNode_acquire_page_token_closure0.v
@@ -17,12 +17,14 @@ Proof.
   all: print_remaining_goal.
   Unshelve. all: sidecond_solver.
   Unshelve. all: sidecond_hammer.
+  (* !start proof(page_allocator.acquire_page_token) *)
   { unfold page_node_can_allocate.
-    revert INV_CASE.
-    destruct (node.(allocation_state)) eqn:Heq; simpl.
-    all: normalize_and_simpl_impl false.
-    all: clear; sidecond_hammer. 
+    opose proof* (page_storage_node_invariant_case_can_allocate) as Heq; first apply INV_CASE.
+    rewrite -Heq. unfold page_node_can_allocate.
+    unfold ord_le.
+    split; solve_goal.
   }
+  (* !end proof *)
 
   Unshelve. all: print_remaining_sidecond.
 Qed.
