verification/rust_proofs/ace/proofs/proof_core_page_allocator_allocator_PageStorageTreeNode_store_page_token_in_this_node.v
@@ -15,15 +15,19 @@ Proof.
   core_page_allocator_allocator_PageStorageTreeNode_store_page_token_in_this_node_prelude.
 
   rep liRStep; liShow.
-  { liInst Hevar (mk_page_node self.(max_node_size) self.(base_address) PageTokenAvailable self.(children_initialized)).
+  (* !start proof(page_allocator.store_page_token_in_this_node) *)
+  { liInst Hevar_rf (mk_page_node self.(max_node_size) self.(base_address) PageTokenAvailable self.(children_initialized)).
     rep liRStep; liShow. }
+  (* !end proof *)
 
   all: print_remaining_goal.
   Unshelve. all: sidecond_solver.
   Unshelve. all: sidecond_hammer.
+  (* !start proof(page_allocator.store_page_token_in_this_node) *)
   { move: INV_CASE.
     unfold name_hint. unfold page_storage_node_invariant_case.
     solve_goal. }
+  (* !end proof *)
 
   Unshelve. all: print_remaining_sidecond.
 Qed.
