verification/rust_proofs/ace/proofs/proof_core_page_allocator_allocator_PageStorageTreeNode_try_to_merge_page_tokens.v
@@ -1,0 +1,153 @@
+From caesium Require Import lang notation.
+From refinedrust Require Import typing shims.
+From sm.ace.generated Require Import generated_code_ace generated_specs_ace generated_template_core_page_allocator_allocator_PageStorageTreeNode_try_to_merge_page_tokens.
+
+Set Default Proof Using "Type".
+
+Section proof.
+Context `{RRGS : !refinedrustGS Σ}.
+
+Lemma core_page_allocator_allocator_PageStorageTreeNode_try_to_merge_page_tokens_proof (π : thread_id) :
+  core_page_allocator_allocator_PageStorageTreeNode_try_to_merge_page_tokens_lemma π.
+Proof.
+  core_page_allocator_allocator_PageStorageTreeNode_try_to_merge_page_tokens_prelude.
+
+  rep <-! liRStep; liShow.
+  (* !start proof(page_allocator.try_to_merge_page_tokens) *)
+  rep liRStep; liShow.
+  { liInst Hevar_x2 (λ child, child.(allocation_state) = PageTokenAvailable).
+    rep liRStep. }
+  rep liRStep; liShow.
+  2: { rep liRStep; liShow.
+    liInst Hevar_rf (mk_page_node self.(max_node_size) self.(base_address) self.(allocation_state) true).
+    rep liRStep; liShow. }
+  (* picking invariant for map: all nodes emitted by the iterator are available *)
+  liInst Hevar_Inv (λ π iter _, ⌜Forall (λ node, node.(allocation_state) = PageTokenAvailable) iter.*1⌝%I).
+
+  rep <-! liRStep; liShow.
+
+  iRename select (IteratorNextFusedTrans _ _ _ _ _ _) into "Hiter".
+  iPoseProof (iterator_next_fused_trans_map_inv with "Hiter") as "Hiter".
+  simpl.
+  set (new_children := (fmap (λ child, {| max_node_size := max_node_size child; base_address := base_address child; allocation_state := PageTokenUnavailable; children_initialized := children_initialized child |}) x')).
+  iApply updateable_add_fupd.
+  iAssert (|={⊤}=> ObsList x'0 new_children)%I with "[Hiter]" as "Hobs" .
+  { iDestruct "Hiter" as "(%hist' & % & _ & _ & _ & Hiter & Hpred)".
+    iMod (learn_from_hyp_proof with "[] Hiter") as "(_ & Hb)"; first done.
+    simpl. rewrite right_id. iDestruct "Hb" as "<-".
+    rewrite big_sepL2_fmap_r.
+    (* TODO: we should simplify Hpred using some big_sepL2 simplification machinery similar to the Forall2 machinery *)
+    iPoseProof (big_sepL2_impl _ (λ _ child _,
+      Obs child.2 {| max_node_size := max_node_size child.1; base_address := base_address child.1; allocation_state := PageTokenUnavailable; children_initialized := children_initialized child.1 |}) with "Hpred []")%I as "Ha".
+    { iModIntro. iIntros (? ? ???). iIntros "(% & % & % & % & % & _ & _ & %child & % & -> & -> & %Heq & (%ret & <- & % & % & Hobs & ->) & _)".
+      injection Heq. intros ->. done. }
+    iPoseProof (big_sepL2_elim_r with "Ha") as "Ha".
+    (*iPoseProof (big_sepL2_from_zip with "Ha") as "Ha".*)
+    rewrite /ObsList. 
+    iApply big_sepL2_from_zip. { rewrite /new_children length_fmap//. }
+    rewrite zip_flip big_sepL_fmap. rewrite zip_fmap_r big_sepL_fmap.
+    iApply (big_sepL_impl with "Ha").
+    iModIntro. iModIntro. iIntros (? [] ?). simpl. eauto. }
+  iMod "Hobs". iModIntro.
+
+  rep liRStep; liShow.
+  liInst Hevar_rf (mk_page_node self.(max_node_size) self.(base_address) PageTokenAvailable true).
+  rep liRStep; liShow.
+
+  all: print_remaining_goal.
+  Unshelve. all: sidecond_solver.
+  Unshelve. all: sidecond_hammer.
+  all: try rename x'1 into children.
+  all: try rename l3 into tokens.
+  all: try rename select (Forall2 _ _ tokens) into Hf.
+  all: rewrite Hchild_init in INV_INIT_CHILDREN.
+  all: try (opose proof * Forall2_length as Hlen; first apply Hf).
+  - eexists. done.
+  - move: INV_CASE.
+    rename select (children_initialized self = true) into Hchild_init.
+    destruct self. simpl in *.
+    rewrite Hchild_init. done.
+  - rewrite -Hlen length_zip. lia.
+  - rewrite length_zip Nat.min_l in Hlen; last lia.
+    specialize (page_size_multiplier_ge (max_node_size self)) as Hge.
+    odestruct (lookup_lt_is_Some_2 tokens 0 _) as (tok0 & Hlook_tok0).
+    { lia. }
+    rewrite snd_zip; last solve_goal.
+    erewrite list_lookup_total_correct; last done.
+    opose proof* Forall2_lookup_r as Hlook1; [apply Hf | apply Hlook_tok0 | ].
+    destruct Hlook1 as ([child_node0 ?] & Hlook_child & _ & Hsz & Hloc).
+    apply lookup_zip_Some in Hlook_child as [Hlook_child _].
+    destruct INV_WF as [INV_WF _].
+    opose proof (INV_WF _ _ 0%nat _ _) as Hchild; [done | done | ].
+    destruct Hchild as (Hchild_sz & Hchild_addr & _).
+    rewrite /aligned_to.
+    rewrite Hloc/=.
+    rewrite Hchild_addr.
+    rewrite /child_base_address/=.
+    rewrite Z.mul_0_r Z.add_0_r.
+    eexists. done.
+  - rename select (_ !! i = Some pg) into Htok_i.
+    rewrite snd_zip in Htok_i; last lia.
+    opose proof* Forall2_lookup_r as Hlook1; [apply Hf | apply Htok_i | ].
+    destruct Hlook1 as ([child_node ?] & Hlook_child & _ & Hsz & Hloc).
+    apply lookup_zip_Some in Hlook_child as [Hlook_child _].
+    destruct INV_WF as [INV_WF _].
+    opose proof (INV_WF _ _ i _ _) as Hchild; [done | done | ].
+    destruct Hchild as (Hchild_sz & Hchild_addr & _).
+    rewrite Hsz Hchild_sz//.
+  - (* use invariant *)
+    rewrite length_zip Nat.min_l in Hlen; last lia.
+    specialize (page_size_multiplier_ge (max_node_size self)) as Hge.
+    odestruct (lookup_lt_is_Some_2 tokens 0 _) as (tok0 & Hlook_tok0).
+    { lia. }
+    rewrite snd_zip; last solve_goal.
+    erewrite list_lookup_total_correct; last done.
+    opose proof* Forall2_lookup_r as Hlook1; [apply Hf | apply Hlook_tok0 | ].
+    destruct Hlook1 as ([child_node0 ?] & Hlook_child & _ & Hsz & Hloc).
+    apply lookup_zip_Some in Hlook_child as [Hlook_child _].
+
+    rename select (_ !! i = Some _) into Htok_i.
+    rewrite snd_zip in Htok_i; last solve_goal.
+    opose proof* Forall2_lookup_r as Hlook2; [apply Hf | apply Htok_i | ].
+    destruct Hlook2 as ([child_nodei ?] & Hlook_child_i & _ & Hsz' & Hloc').
+    apply lookup_zip_Some in Hlook_child_i as [Hlook_child_i _].
+
+    destruct INV_WF as [INV_WF _].
+    opose proof (INV_WF _ _ i _ _) as Hchild; [done | done | ].
+    destruct Hchild as (Hchild_sz & Hchild_addr & _).
+
+    opose proof (INV_WF _ _ 0%nat _ _) as Hchild; [done | done | ].
+    destruct Hchild as (Hchild_sz_0 & Hchild_addr_0 & _).
+
+    rewrite Hloc'/= Hchild_addr Hloc/=.
+    rewrite Hchild_addr_0.
+    rewrite Hsz' Hchild_sz.
+    rewrite /child_base_address.
+    simpl. clear. nia.
+  - apply page_storage_node_children_wf_upd_state; last done.
+    simpl. solve_goal.
+  - eexists. done.
+  - rewrite /new_children length_fmap//.
+  - rewrite /page_storage_node_invariant_case/=.
+    eexists. split_and!; try done. simpl.
+    rewrite length_zip Nat.min_l in Hlen; last lia.
+    specialize (page_size_multiplier_ge (max_node_size self)) as Hge.
+    odestruct (lookup_lt_is_Some_2 tokens 0 _) as (tok0 & Hlook_tok0).
+    { lia. }
+    rewrite snd_zip; last solve_goal.
+    erewrite list_lookup_total_correct; last done.
+    opose proof* Forall2_lookup_r as Hlook1; [apply Hf | apply Hlook_tok0 | ].
+    destruct Hlook1 as ([child_node0 ?] & Hlook_child & _ & Hsz & Hloc).
+    apply lookup_zip_Some in Hlook_child as [Hlook_child _].
+    destruct INV_WF as [INV_WF _].
+    opose proof (INV_WF _ _ 0%nat _ _) as Hchild; [done | done | ].
+    destruct Hchild as (Hchild_sz & Hchild_addr & _).
+    rewrite Hloc/=.
+    rewrite Hchild_addr.
+    rewrite /child_base_address/=.
+    rewrite Z.mul_0_r Z.add_0_r//.
+  (* !end proof *)
+
+  Unshelve. all: print_remaining_sidecond.
+Qed.
+End proof.
