verification/rust_proofs/ace/proofs/proof_core_page_allocator_page_Page_T_write.v
@@ -7,15 +7,13 @@ Set Default Proof Using "Type".
 Section proof.
 Context `{RRGS : !refinedrustGS Σ}.
 
-Global Instance bla_copy : Copyable (error_Error_ty <INST!>).
-Proof. apply _. Qed.
-
 Lemma core_page_allocator_page_Page_T_write_proof (π : thread_id) :
   core_page_allocator_page_Page_T_write_lemma π.
 Proof.
   core_page_allocator_page_Page_T_write_prelude.
 
   rep <-! liRStep; liShow.
+  (* !start proof(page.write) *)
   {
     rename select (offset_in_bytes `rem` 8 = 0) into Hoffset.
     apply Z.rem_divide in Hoffset; last done.
@@ -27,10 +25,12 @@ Proof.
   }
   { rep liRStep; liShow. }
   { rep liRStep; liShow. }
+  (* !end proof *)
 
   all: print_remaining_goal.
   Unshelve. all: sidecond_solver.
   Unshelve. all: sidecond_hammer.
+  (* !start proof(page.write) *)
   {
     revert select (_ + off' * 8 < _ + page_size_in_bytes_Z _).
     rewrite /page_size_in_bytes_nat.
@@ -47,6 +47,7 @@ Proof.
     rename select (offset_in_bytes `rem` 8 ≠ 0) into Hen.
     apply Hen. unfold name_hint in *.
     apply Z.rem_divide; done. }
+  (* !end proof *)
 
   Unshelve. all: print_remaining_sidecond.
 Qed.
