verification/rust_proofs/pointers_utility/proofs/proof_ptr_byte_add_mut.v
@@ -17,26 +17,27 @@ Proof.
   all: print_remaining_goal.
   Unshelve. all: sidecond_solver.
   Unshelve. all: sidecond_hammer.
-    
-  all: try rename select ((wrap_unsigned (pointer.2 + offset_in_bytes) usize ?= owned_region_end.2) = Lt) into Hwrap_lt.
-  all: try rewrite Z.compare_lt_iff in Hwrap_lt.
-  all: try rename select (wrap_unsigned (pointer.2 + offset_in_bytes) usize ≤ pointer.2) into Hoverflow.
-  { opose proof (wrap_unsigned_le (pointer.2 + offset_in_bytes) usize _); lia. } 
+
+  (* !start proof(pointers_utility.ptr_byte_add_mut) *)
+  all: try rename select ((wrap_unsigned (pointer.(loc_a) + offset_in_bytes) usize < owned_region_end.(loc_a))) into Hwrap_lt.
+  all: try rename select (wrap_unsigned (pointer.(loc_a) + offset_in_bytes) usize ≤ pointer.(loc_a)) into Hoverflow.
+  { opose proof (wrap_unsigned_le (pointer.(loc_a) + offset_in_bytes) usize _); lia. }
   { apply wrap_unsigned_add_did_wrap in Hoverflow; [ | done.. | lia].
     sidecond_hammer.
   }
-  { rewrite wrap_unsigned_add_did_not_wrap in Hwrap_lt; sidecond_hammer. } 
+  { rewrite wrap_unsigned_add_did_not_wrap in Hwrap_lt; sidecond_hammer. }
   { rewrite wrap_unsigned_add_did_not_wrap in Hwrap_lt; [ | sidecond_hammer..].
     apply wrapping_shift_loc_shift_loc.
     sidecond_hammer.
-  } 
+  }
   { (* offset is zero. So this is okay. *)
     assert (offset_in_bytes = 0) as -> by lia.
     rewrite Z.add_0_r in Hwrap_lt.
     rewrite wrap_unsigned_id in Hwrap_lt; [ lia | done..  ]. }
   { assert (offset_in_bytes = 0) as -> by lia.
     rewrite shift_loc_0 wrapping_shift_loc_0//. }
+  (* !end proof *)
 
   Unshelve. all: print_remaining_sidecond.
-Admitted. (* admitted due to admit_proofs config flag *)
+Qed.
 End proof.
