verification/theories/memory_layout/memory_layout.v
@@ -2,16 +2,17 @@ From refinedrust Require Import typing.
 
 (** * Additional definitions for the security monitor's global memory layout *)
 
+(* !start spec(memory_layout.memory_layout) *)
 Record memory_layout : Type := mk_memory_layout {
   conf_start : loc;
   conf_end : loc;
   non_conf_start : loc;
   non_conf_end : loc;
 
-  conf_start_in_usize : conf_start.2 ∈ usize;
-  conf_end_in_usize : conf_end.2 ∈ usize;
-  non_conf_start_in_usize : non_conf_start.2 ∈ usize;
-  non_conf_end_in_usize : non_conf_end.2 ∈ usize;
+  conf_start_in_usize : conf_start.(loc_a) ∈ usize;
+  conf_end_in_usize : conf_end.(loc_a) ∈ usize;
+  non_conf_start_in_usize : non_conf_start.(loc_a) ∈ usize;
+  non_conf_end_in_usize : non_conf_end.(loc_a) ∈ usize;
 }.
 Canonical Structure memory_layoutRT := directRT memory_layout. 
 
@@ -19,3 +20,4 @@ Global Program Instance memory_layout_inhabited : Inhabited memory_layout :=
   populate (mk_memory_layout 
     NULL_loc NULL_loc NULL_loc NULL_loc _ _ _ _).
 Solve Obligations with split; unsafe_unfold_common_caesium_defs; sidecond_hammer.
+(* !end spec *)
